theories/diffpriv/examples/exact_cache.v
@@ -1,33 +1,33 @@
-(* From iris.base_logic Require Export na_invariants. *)
-(* From clutch.common Require Import inject. *)
-(* From clutch.prelude Require Import tactics. *)
-(* From clutch.prob Require Import differential_privacy. *)
-(* From clutch.diffpriv Require Import adequacy diffpriv proofmode. *)
-(* From clutch.diffpriv.examples Require Import list map. *)
+From iris.base_logic Require Export na_invariants.
+From clutch.common Require Import inject.
+From clutch.prelude Require Import tactics.
+From clutch.prob Require Import differential_privacy.
+From clutch.diffpriv Require Import adequacy diffpriv proofmode.
+From clutch.diffpriv.examples Require Import list map.
 
-(* Section xcache. *)
-(*   Context `{!diffprivGS Σ}. *)
+Section xcache.
+  Context `{!diffprivGS Σ}.
 
-(*   #[local] Open Scope R. *)
+  #[local] Open Scope R.
 
-(*   (* TODO instantiate exact_cache with a mechanism *) *)
+  (* TODO instantiate exact_cache with a mechanism *)
 
-(*   (* SPEC: If M is ε-dp, then exact_cache M qs is kε-dp where k = |unique(qs)|. *) *)
-(*   Definition exact_cache : val := *)
-(*     λ:"M" "qs" "db", *)
-(*       let: "cache" := init_map #() in *)
-(*       list_fold *)
-(*         (λ: "acc" "q", *)
-(*            match: get "cache" "q" with *)
-(*            | SOME "v" => list_cons "v" "acc" *)
-(*            | NONE => *)
-(*                let: "v" := "M" "q" "db" in *)
-(*                set "cache" "q" "v" ;; *)
-(*                list_cons "v" "acc" *)
-(*            end) *)
-(*         list_nil "qs". *)
+  (* SPEC: If M is ε-dp, then exact_cache M qs is kε-dp where k = |unique(qs)|. *)
+  Definition exact_cache : val :=
+    λ:"M" "qs" "db",
+      let: "cache" := init_map #() in
+      list_fold
+        (λ: "acc" "q",
+           match: get "cache" "q" with
+           | SOME "v" => list_cons "v" "acc"
+           | NONE =>
+               let: "v" := "M" "q" "db" in
+               set "cache" "q" "v" ;;
+               list_cons "v" "acc"
+           end)
+        list_nil "qs".
 
-(*   (* Given a set of queries qs and a ε-dp mechanism M, exact_cache M qs is kε-dp where k=|qs|. *)
+  (* Given a set of queries qs and a ε-dp mechanism M, exact_cache M qs is kε-dp where k=|qs|. *)
 
 (*     To enable caching we need decidable equality on the type of queries, so *)
 (*     we'll just work with integers (think of this as the Gödel encoding of the *)
@@ -48,434 +48,487 @@
 (*     well decode q into a sensitive query function and add noise to the result *)
 (*     of the query to achieve this privacy guarantee. *)
 
-(*    *) *)
+(*    *)
 
-(*   Definition online_xcache : val := *)
-(*     λ:"M" "db", *)
-(*       let: "cache" := init_map #() in *)
-(*       (λ: "q", *)
-(*          match: get "cache" "q" with *)
-(*          | SOME "v" => "v" *)
-(*          | NONE => let: "v" := "M" "q" "db" in *)
-(*                    set "cache" "q" "v" ;; *)
-(*                    "v" *)
-(*          end). *)
+  Definition online_xcache : val :=
+    λ:"M" "db",
+      let: "cache" := init_map #() in
+      (λ: "q",
+         match: get "cache" "q" with
+         | SOME "v" => "v"
+         | NONE => let: "v" := "M" "q" "db" in
+                   set "cache" "q" "v" ;;
+                   "v"
+         end).
 
-(*   (* We can define the original exact_cache as a client of the online spec (keeping the direct def.) *) *)
-(*   Definition exact_cache_offline_map : val := *)
-(*     λ:"M" "qs" "db", *)
-(*       let: "oXC" := online_xcache "M" "db" in *)
-(*       list_map "oXC" "qs". *)
+  (* We can define the original exact_cache as a client of the online spec (keeping the direct def.) *)
+  Definition exact_cache_offline_map : val :=
+    λ:"M" "qs" "db",
+      let: "oXC" := online_xcache "M" "db" in
+      list_map "oXC" "qs".
 
-(*   (* Same but with list_fold (used in one proof) *) *)
-(*   Definition exact_cache_offline : val := *)
-(*     λ:"M" "qs" "db", *)
-(*       let: "oXC" := online_xcache "M" "db" in *)
-(*       list_fold (λ: "acc" "q", list_cons ("oXC" "q") "acc") list_nil "qs". *)
+  (* Same but with list_fold (used in one proof) *)
+  Definition exact_cache_offline : val :=
+    λ:"M" "qs" "db",
+      let: "oXC" := online_xcache "M" "db" in
+      list_fold (λ: "acc" "q", list_cons ("oXC" "q") "acc") list_nil "qs".
 
-(*   Definition oxc_spec0_cached (f f' : val) (F : gmap nat val → iProp Σ) : iProp Σ := *)
-(*     (∀ (q : nat) A K, *)
-(*         ⌜q ∈ dom A⌝ -∗ *)
-(*         F(A) -∗ *)
-(*         ⤇ fill K (Val f' #q) -∗ *)
-(*         WP (Val f) #q {{ v, F(A) ∗ ⤇ fill K (Val v) ∗  ⌜A !! q = Some v⌝ }}). *)
+  Definition oxc_spec0_cached `{Inject A val} (eqA : Equiv A) (f f' : val) (F : gmap nat A → gmap nat A → iProp Σ) : iProp Σ :=
+    (∀ (q : nat) (m m' : gmap nat A) K,
+        ⌜m ≡ m'⌝ -∗
+        ⌜q ∈ dom m⌝ -∗
+        F m m' -∗
+        ⤇ fill K (Val f' #q) -∗
+        WP (Val f) #q {{ v, ∃ (a a' : A), ⌜v = inject a⌝ ∗ ⌜a ≡ a'⌝ ∗ F m m' ∗ ⤇ fill K (inject a') ∗  ⌜m !! q = Some a⌝ }}).
 
-(*   Definition oxc_spec0_fresh (M : val) c `(dDB : Distance DB) (f f' : val) (F : gmap nat val → iProp Σ) : iProp Σ := *)
-(*     (∀ (q : nat) A ε δ K, *)
-(*         ⌜q ∉ dom A⌝ -∗ *)
-(*         wp_diffpriv (M #q) ε δ dDB -∗ *)
-(*         ↯m (c * ε) -∗ *)
-(*         ↯ (c * δ) -∗ *)
-(*         F(A) -∗ *)
-(*         ⤇ fill K (Val f' #q) -∗ *)
-(*         WP (Val f) #q {{ v, F( <[q := v]> A) ∗ ⤇ fill K (Val v) }}). *)
-
-
-(*   #[local] Definition exact_cache_body {DB} {dDB : Distance DB} (M : val) (db : DB) (cache_loc : loc) : expr := *)
-(*     ((λ: "acc" "q", *)
-(*         match: get #cache_loc "q" with *)
-(*           InjL <> => *)
-(*             let: "v" := M "q" (inject db) in *)
-(*             set #cache_loc "q" "v";; list_cons "v" "acc" *)
-(*         | InjR "v" => list_cons "v" "acc" *)
-(*         end)%V). *)
-
-(*   (* Direct proof via Löb induction for the definition with fold. *) *)
-(*   Lemma exact_cache_dipr (M : val) DB (dDB : Distance DB) (qs : list nat) (QS : val) (is_qs : is_list qs QS) *)
-(*     ε δ (εpos : 0 <= ε) (δpos : 0 <= δ) *)
-(*     (M_dipr : Forall (λ q : nat, ⊢ hoare_diffpriv (M #q) ε δ dDB) qs) *)
-(*     : *)
-(*     let k := size ((list_to_set qs) : gset _) in *)
-(*     ⊢ hoare_diffpriv (exact_cache M QS) (k*ε) (k*δ) dDB. *)
-(*   Proof with (tp_pures ; wp_pures). *)
-(*     iIntros (k K c db db' adj φ) "!> [rhs ε] hφ". rewrite {2}/exact_cache... *)
-(*     wp_apply wp_init_map => // ; iIntros (cache_l) "cache_l"... *)
-(*     rewrite /exact_cache... tp_bind (init_map _). *)
-(*     iMod (spec_init_map with "rhs") as "(%cache_r & rhs & cache_r)" => /=... *)
-(*     rewrite -!/(exact_cache_body _ _ _). *)
-(*     revert qs QS is_qs k M_dipr. *)
-(*     cut *)
-(*       (∀ (qs : list nat) *)
-(*          (qs_pre qs' : list nat) (QS' : val) *)
-(*          (acc : val) cache_map, *)
-(*           qs = qs_pre ++ qs' → *)
-(*           dom cache_map = list_to_set qs_pre → *)
-(*           dom cache_map ∪ list_to_set qs' = list_to_set qs → *)
-(*           is_list qs' QS' → *)
-(*           Forall (λ q : nat, ⊢ hoare_diffpriv (M #q) ε δ dDB) qs → *)
-(*           let k := size (list_to_set qs : gset nat) in *)
-(*           let k' := size cache_map in *)
-(*           {{{ *)
-(*                 ↯m (c * ((k - k') * ε)) ∗ ↯ (c * ((k - k') * δ)) *)
-(*                 ∗ ⤇ fill K (list_fold (exact_cache_body M db' cache_r) acc QS') *)
-(*                 ∗ map_list cache_l cache_map *)
-(*                 ∗ map_slist cache_r cache_map *)
-(*           }}} *)
-(*             list_fold (exact_cache_body M db cache_l) acc QS' *)
-(*             {{{ vl, RET vl ; ∃ (vr : val), ⤇ fill K vr ∗ ⌜vl = vr⌝ }}} *)
-(*       ). *)
-(*     { *)
-(*       intros h. intros. iApply (h qs [] qs QS _ ∅ with "[-hφ]") => //. *)
-(*       1: set_solver. *)
-(*       2: iNext ; iIntros (?) "(% & ? & ->)" ; iApply "hφ" => //. *)
-(*       iFrame. rewrite map_size_empty. rewrite Rminus_0_r. subst k. simpl. iFrame. *)
-(*     } *)
-(*     clear φ. *)
-(*     iLöb as "IH". *)
-(*     iIntros (qs qs_pre qs' QS' acc cache qs_pre_qs' dom_cache_pre dom_cache_qs'_qs is_qs' *)
-(*                M_dipr φ) "(ε & δ & rhs & cache_l & cache_r) hφ". *)
-(*     set (k := size (list_to_set qs : gset nat)). *)
-(*     set (k' := size cache). *)
-(*     rewrite {4}/exact_cache_body/list_fold... rewrite -!/(exact_cache_body _ _ _) -/list_fold. *)
-(*     destruct qs' as [|q' qs''] eqn:qs'_qs''. *)
-(*     1:{ rewrite is_qs'. rewrite {3}/exact_cache_body/list_fold... iApply "hφ". iExists _. iFrame => //. } *)
-(*     rewrite {3}/exact_cache_body/list_fold... rewrite -!/(exact_cache_body _ _ _) -/list_fold. *)
-(*     destruct is_qs' as (QS'' & -> & is_qs'')... *)
-(*     wp_apply (wp_get with "cache_l"). iIntros (?) "[cache_l ->]". *)
-(*     tp_bind (get _ _). iMod (spec_get with "cache_r rhs") as "[rhs cache_r]" => /=. *)
-(*     rewrite -!/(exact_cache_body _ _ _) -/list_fold. *)
-(*     rewrite qs_pre_qs' in M_dipr. *)
-(*     destruct ((proj1 (List.Forall_app _ _ _)) M_dipr) as [M_dipr_qs_pre M_dipr_qs']. *)
-(*     destruct (Forall_cons_1 _ _ _ M_dipr_qs') as [M_dipr_q' M_dipr_qs'']. *)
-(*     assert (0 <= dDB db db') by apply distance_pos. *)
-(*     destruct (cache !! q') eqn:cache_q' => /=. *)
-(*     - opose proof (elem_of_dom_2 _ _ _ cache_q') as h... *)
-(*       rewrite /list_cons. do 7 wp_pure. do 7 tp_pure. *)
-(*       rewrite -!/(exact_cache_body _ _ _) -/list_fold. *)
-(*       iSpecialize ("IH" $! qs (qs_pre ++ [q']) qs'' QS'' (InjRV (v, acc)) cache). *)
-(*       unshelve iApply ("IH" $! _ _ _ _ _ _ with "[$ε $δ $rhs $cache_l $cache_r]") => //. *)
-(*       1: subst ; by rewrite cons_middle assoc. *)
-(*       all: subst ; assumption || set_solver. *)
-(*     - opose proof (not_elem_of_dom_2 _ _ cache_q') as h... *)
-(*       tp_bind (M _ _). wp_bind (M _ _). *)
-(*       assert ((c * ((k - k') * ε)) = (c * (k - (k'+1)) * ε + c * ε)) as -> by lra. *)
-(*       assert ((c * ((k - k') * δ)) = (c * (k - (k'+1)) * δ + c * δ)) as -> by lra. *)
-(*       assert (0 <= k - (k' + 1)). *)
-(*       { *)
-(*         subst. subst k k'. apply Rle_0_le_minus. *)
-(*         rewrite -dom_cache_qs'_qs. *)
-(*         replace (size cache) with (size (dom cache)) by apply size_dom. *)
-(*         rewrite dom_cache_pre. replace 1 with (INR 1) by auto. *)
-(*         replace 1%nat with (size (list_to_set [q'] : gset nat)). *)
-(*         2:{ cbn. rewrite union_empty_r_L. apply size_singleton. } *)
-(*         rewrite -plus_INR. rewrite -size_union. 2: set_solver. *)
-(*         rewrite (list_to_set_cons _ qs''). simpl. *)
-(*         apply le_INR. apply subseteq_size. set_solver. *)
-(*       } *)
-(*       iDestruct (ecm_split with "ε") as "[kε ε]". 2: real_solver. 1: repeat real_solver_partial => //. *)
-(*       iDestruct (ec_split with "δ") as "[kδ δ]". 2: real_solver. 1: repeat real_solver_partial => //. *)
-(*       iApply (M_dipr_q' with "[] [rhs ε δ]") => // ; iFrame. iNext. iIntros (vq') "rhs" => /=... *)
-(*       tp_bind (set _ _ _). iMod (spec_set with "cache_r rhs") as "[rhs cache_r]". *)
-(*       wp_apply (wp_set with "cache_l") ; iIntros "cache_l"... *)
-(*       rewrite /list_cons. do 7 wp_pure. simpl. do 9 tp_pure. *)
-(*       iSpecialize ("IH" $! qs (qs_pre ++ [q']) qs'' QS'' (InjRV (vq', acc)) _). *)
-(*       iSpecialize ("IH" $! _ _ _ _ _ _ with "[kε kδ $rhs $cache_l $cache_r]") => //. *)
-(*       2: iApply "IH" => //. *)
-(*       iSplitL "kε". *)
-(*       + iApply ecm_eq. 2: iFrame. real_solver_partial. subst k. simpl. subst k'. *)
-(*         replace (INR $ size (<[q' := vq']> cache)) with (size cache + 1) => //. *)
-(*         rewrite map_size_insert_None => //. qify_r ; zify_q. lia. *)
-(*       + iApply ec_eq. 2: iFrame. real_solver_partial. subst k. simpl. subst k'. *)
-(*         replace (INR $ size (<[q' := vq']> cache)) with (size cache + 1) => //. *)
-(*         rewrite map_size_insert_None => //. qify_r ; zify_q. lia. *)
-(*         Unshelve. *)
-(*         1: subst ; by rewrite cons_middle assoc. *)
-(*         all: subst ; assumption || set_solver. *)
-(*   Qed. *)
-
-(*   (* pay as you go, cache map exposed, M only needs to be private on the queries it gets executed on *) *)
-(*   Lemma oxc_spec0 (M : val) `(dDB : Distance DB) (db db' : DB) c (adj : dDB db db' <= c) K : *)
-(*     ⤇ fill K (online_xcache M (Val (inject db'))) *)
-(*     ⊢ WP online_xcache M (Val (inject db)) *)
-(*         {{ f, ∃ f', ⤇ fill K (Val f') ∗ *)
-(*                     ∃ (F : gmap nat val → iProp Σ), *)
-(*                       F ∅ ∗ *)
-(*                       □ oxc_spec0_cached f f' F ∗ *)
-(*                       □ oxc_spec0_fresh M c dDB f f' F *)
-(*         }}. *)
-(*   Proof with (tp_pures ; wp_pures). *)
-(*     iIntros "rhs". rewrite /online_xcache... *)
-(*     tp_bind (init_map _). iMod (spec_init_map with "rhs") as "[%cache_r [rhs cache_r]]". *)
-(*     simpl... wp_apply wp_init_map => //. iIntros (cache_l) "?"... *)
-(*     iModIntro. iExists _. iFrame "rhs". *)
-(*     iExists (λ A, map_list cache_l A ∗ map_slist cache_r A)%I. *)
-(*     iFrame. iSplit. *)
-(*     - iIntros "!>" (??? cached) "[cache_l cache_r] rhs"... *)
-(*       tp_bind (get _ _). iMod (spec_get with "[$cache_r] [$rhs]") as "[rhs cache_r]". *)
-(*       wp_apply (wp_get with "cache_l") ; iIntros (vq) "[cache_l %hvq]". *)
-(*       simpl. subst. apply elem_of_dom in cached. rewrite /opt_to_val. *)
-(*       destruct cached as [vq hvq]. rewrite hvq. tp_pures. wp_pures. iFrame. done. *)
-(*     - iIntros "!>" (????? cached) "M_dipr ε δ [cache_l cache_r] rhs"... *)
-(*       tp_bind (get _ _). iMod (spec_get with "[$cache_r] [$rhs]") as "[rhs cache_r]". *)
-(*       wp_apply (wp_get with "cache_l") ; iIntros (vq) "[cache_l %hvq]". *)
-(*       simpl. subst. apply not_elem_of_dom_1 in cached. rewrite /opt_to_val. *)
-(*       rewrite !cached... tp_bind (M _ _). wp_bind (M _ _). *)
-(*       rewrite /wp_diffpriv. iSpecialize ("M_dipr" $! _ c db db' adj). *)
-(*       iSpecialize ("M_dipr" with "[$rhs $ε $δ]"). *)
-(*       iApply (wp_strong_mono'' with "M_dipr"). iIntros (vq) "rhs" => /=... *)
-(*       tp_bind (set _ _ _). iMod (spec_set with "[$cache_r] [$rhs]") as "[rhs cache_r]". *)
-(*       wp_apply (wp_set with "cache_l") ; iIntros "cache_l". *)
-(*       simpl. tp_pures. wp_pures. by iFrame. *)
-(*   Qed. *)
-
-(*   (* we can derive spec1 from spec0 *) *)
-(*   (* F can store error credits ; could also ask for N*ε error credits upfront and hand out F(∅, N) instead of F(∅, 0). *) *)
-(*   Lemma oxc_spec1 (M : val) `(dDB : Distance DB) (db db' : DB) (adj : dDB db db' <= 1) K ε δ (εpos : 0 <= ε) (δpos : 0 <= δ) : *)
-(*     (∀ q : nat, hoare_diffpriv (M #q) ε δ dDB) ∗ *)
-(*     ⤇ fill K (online_xcache M (Val (inject db'))) *)
-(*     ⊢ WP online_xcache M (Val (inject db)) *)
-(*         {{ f, ∃ f', ⤇ fill K (Val f') ∗ *)
-(*                     ∃ (F : gmap nat val * nat → iProp Σ), *)
-(*                       F (∅, 0%nat) ∗ *)
-(*                       □ (∀ A k, ↯m ε ∗ ↯ δ ∗ F(A, k) -∗ F(A, S k)) ∗ *)
-(*                       □ (∀ (q : nat) A K (N : nat), *)
-(*                             ⌜q ∈ dom A⌝ -∗ *)
-(*                             F(A, N) -∗ *)
-(*                             ⤇ fill K (Val f' #q) -∗ *)
-(*                             WP (Val f) #q {{ v, F(A, N) ∗ ⤇ fill K (Val v) ∗  ⌜A !! q = Some v⌝ }}) ∗ *)
-(*                       □ (∀ (q : nat) A K (N : nat), *)
-(*                             ⌜q ∉ dom A⌝ -∗ *)
-(*                             F(A, S N) -∗ *)
-(*                             ⤇ fill K (Val f' #q) -∗ *)
-(*                             WP (Val f) #q {{ v, F( <[q := v]> A, N) ∗ ⤇ fill K (Val v) }}) *)
-(*         }}. *)
-(*   Proof with (tp_pures ; wp_pures). *)
-(*     iIntros "(#M_dipr & rhs)". iPoseProof (oxc_spec0 with "[rhs]") as "spec0" => //. *)
-(*     iMod ecm_zero as "ε0" ; iMod ec_zero as "δ0". *)
-(*     iApply (wp_strong_mono'' with "spec0"). iIntros "%f (%f' & rhs & (%F & F0 & #f_cached & #f_fresh))". *)
-(*     iExists f'. iFrame "rhs". *)
-(*     iExists (λ Ak : gmap nat val * nat, let (A, k) := Ak in F A ∗ ↯m (k * ε) ∗ ↯ (k * δ))%I. *)
-(*     rewrite !Rmult_0_l. iFrame "F0 ε0 δ0". *)
-(*     iSplitR ; [|iSplitL "f_cached"]. *)
-(*     - iIntros "!>" (??) "(ε&δ&?&kε&kδ)". iFrame. iPoseProof (ecm_combine with "[ε kε]") as "ε" ; iFrame. *)
-(*       iPoseProof (ec_combine with "[δ kδ]") as "δ" ; iFrame. iSplitL "ε". *)
-(*       + iApply ecm_eq. 2: iFrame. replace (S k) with (k+1)%nat by lia. replace (INR (k+1)) with (k+1)%R. *)
-(*         2: real_solver. lra. *)
-(*       + iApply ec_eq. 2: iFrame. replace (S k) with (k+1)%nat by lia. replace (INR (k+1)) with (k+1)%R. *)
-(*         2: real_solver. lra. *)
-(*     - simpl. iIntros "!>" (?????) "[FA [ε δ]] rhs". iSpecialize ("f_cached" with "[] [$FA] [$rhs]") => //. *)
-(*       iApply (wp_strong_mono'' with "f_cached"). iIntros (?) "(FA & rhs & %)". iFrame => //. *)
-(*     - iIntros "!>" (?????) "[FA [ε δ]] rhs". *)
-(*       replace ((S N)) with (N + 1)%nat by lia. replace (INR (N+1)) with (N+1) by real_solver. *)
-(*       rewrite !Rmult_plus_distr_r. rewrite !Rmult_1_l. *)
-(*       iDestruct (ecm_split with "ε") as "[Nε ε]". 1,2: real_solver. *)
-(*       iDestruct (ec_split with "δ") as "[Nδ δ]". 1,2: real_solver. *)
-(*       iSpecialize ("f_fresh" with "[] [] [ε] [δ] [$FA] [$rhs]") => //. *)
-(*       { iIntros (?????) "[??]". iApply ("M_dipr" with "[] [-]") => //. *)
-(*         2: iNext ; iIntros => //. iFrame. } *)
-(*       1,2: rewrite Rmult_1_l => //. *)
-(*       iApply (wp_strong_mono'' with "f_fresh"). *)
-(*       iIntros (?) "(FA & rhs)". iFrame => //. *)
-(*   Qed. *)
-
-(*   (* We can prove exact_cache_dipr from the online spec. The proof is essentially the same as the direct proof. *) *)
-(*   Lemma exact_cache_dipr_offline (M : val) DB (dDB : Distance DB) (qs : list nat) (QS : val) (is_qs : is_list qs QS) *)
-(*     ε δ (εpos : 0 <= ε) (δpos : 0 <= δ) *)
-(*     (M_dipr : Forall (λ q : nat, ⊢ wp_diffpriv (M #q) ε δ dDB) qs) *)
-(*     : *)
-(*     let k := size ((list_to_set qs) : gset _) in *)
-(*     ⊢ wp_diffpriv (exact_cache_offline M QS) (k*ε) (k*δ) dDB. *)
-(*   Proof with (tp_pures ; wp_pures). *)
-(*     iIntros (k K c db db' adj) "[rhs [ε δ]]". *)
-(*     rewrite {2}/exact_cache_offline... *)
-(*     rewrite /exact_cache_offline... *)
-(*     tp_bind (online_xcache _ _). wp_bind (online_xcache _ _). *)
-(*     iPoseProof (oxc_spec0 M _ _ _ _) as "oXC" => //. *)
-(*     iSpecialize ("oXC" with "rhs"). *)
-(*     iApply (wp_strong_mono'' with "oXC"). *)
-(*     iIntros "%f (%f' & rhs & %F & F & #cached & #fresh) /="... *)
-(*     set (exact_cache_offline_body (f : val) := (λ: "acc" "q", list_cons (f "q") "acc")%V). *)
-(*     rewrite -!/(exact_cache_offline_body _). *)
-(*     revert qs QS is_qs k M_dipr. *)
-(*     cut *)
-(*       (∀ (qs : list nat) *)
-(*          (qs_pre qs' : list nat) (QS' : val) *)
-(*          (acc : val) cache_map, *)
-(*           qs = qs_pre ++ qs' → *)
-(*           dom cache_map = list_to_set qs_pre → *)
-(*           dom cache_map ∪ list_to_set qs' = list_to_set qs → *)
-(*           is_list qs' QS' → *)
-(*           Forall (λ q : nat, ⊢ wp_diffpriv (M #q) ε δ dDB) qs → *)
-(*           let k := size (list_to_set qs : gset nat) in *)
-(*           let k' := size cache_map in *)
-(*           {{{ *)
-(*                 ↯m (c * ((k - k') * ε)) ∗ ↯ (c * ((k - k') * δ)) ∗ *)
-(*                 □ oxc_spec0_cached f f' F ∗ *)
-(*                 □ oxc_spec0_fresh M c dDB f f' F ∗ *)
-(*                 ⤇ fill K (list_fold (exact_cache_offline_body f') acc QS') ∗ *)
-(*                 F cache_map *)
-(*           }}} *)
-(*             list_fold (exact_cache_offline_body f) acc QS' *)
-(*             {{{ vl, RET vl ; ∃ (vr : val), ⤇ fill K vr ∗ ⌜vl = vr⌝ }}} *)
-(*       ). *)
-(*     { *)
-(*       intros h. intros. iApply (h qs [] qs QS _ ∅ with "[-]") => //. *)
-(*       1: set_solver. *)
-(*       2: iNext ; iIntros (?) "(% & ? & ->)" ; done. *)
-(*       iFrame. rewrite map_size_empty. rewrite Rminus_0_r. subst k. simpl. iFrame. *)
-(*       iSplit ; done. *)
-(*     } *)
-(*     iLöb as "IH". *)
-(*     iIntros (qs qs_pre qs' QS' acc cache qs_pre_qs' dom_cache_pre dom_cache_qs'_qs is_qs' *)
-(*                M_dipr φ) "(ε & δ & #cached & #fresh & rhs & F) hφ". *)
-(*     set (k := size (list_to_set qs : gset nat)). *)
-(*     set (k' := size cache). *)
-(*     rewrite {4}/exact_cache_offline_body/list_fold... rewrite -!/(exact_cache_offline_body _) -/list_fold. *)
-(*     destruct qs' as [|q' qs''] eqn:qs'_qs''. *)
-(*     1:{ rewrite is_qs'. rewrite {3}/exact_cache_offline_body/list_fold... iApply "hφ". iExists _. iFrame => //. } *)
-(*     destruct is_qs' as (QS'' & -> & is_qs'')... *)
-(*     rewrite -!/(exact_cache_offline_body _) -/list_fold. *)
-(*     rewrite qs_pre_qs' in M_dipr. *)
-(*     destruct ((proj1 (List.Forall_app _ _ _)) M_dipr) as [M_dipr_qs_pre M_dipr_qs']. *)
-(*     destruct (Forall_cons_1 _ _ _ M_dipr_qs') as [M_dipr_q' M_dipr_qs'']. *)
-(*     assert (0 <= dDB db db') by apply distance_pos. *)
-(*     destruct (cache !! q') eqn:cache_q' => /=. *)
-(*     - opose proof (elem_of_dom_2 _ _ _ cache_q') as h... *)
-(*       rewrite /exact_cache_offline_body... *)
-(*       tp_bind (f' _) ; wp_bind (f _). *)
-(*       iCombine "cached" as "h". *)
-(*       iSpecialize ("h" $! q' cache _ h with "F rhs"). *)
-(*       iApply (wp_strong_mono'' with "h"). *)
-(*       iIntros "/= %v' (F & rhs & %cache_q'')". *)
-(*       assert (v = v') as <-. { rewrite cache_q' in cache_q''. inversion cache_q''. done. } *)
-(*       rewrite /list_cons... *)
-(*       rewrite -!/(exact_cache_offline_body _) -/list_fold. *)
-(*       iSpecialize ("IH" $! qs (qs_pre ++ [q']) qs'' QS'' (InjRV (v, acc)) cache). *)
-(*       unshelve iApply ("IH" $! _ _ _ _ _ _ with "[ε δ rhs F]") => //. *)
-(*       1: subst ; by rewrite cons_middle assoc. *)
-(*       all: subst ; try assumption. *)
-(*       1,2: set_solver. iFrame. iSplit ; done. *)
-(*     - opose proof (not_elem_of_dom_2 _ _ cache_q') as h... *)
-(*       assert ((c * ((k - k') * ε)) = (c * (k - (k'+1)) * ε + c * ε)) as -> by lra. *)
-(*       assert ((c * ((k - k') * δ)) = (c * (k - (k'+1)) * δ + c * δ)) as -> by lra. *)
-(*       assert (0 <= k - (k' + 1)). *)
-(*       { *)
-(*         subst. subst k k'. apply Rle_0_le_minus. *)
-(*         rewrite -dom_cache_qs'_qs. *)
-(*         replace (size cache) with (size (dom cache)) by apply size_dom. *)
-(*         rewrite dom_cache_pre. replace 1 with (INR 1) by auto. *)
-(*         replace 1%nat with (size (list_to_set [q'] : gset nat)). *)
-(*         2:{ cbn. rewrite union_empty_r_L. apply size_singleton. } *)
-(*         rewrite -plus_INR. rewrite -size_union. 2: set_solver. *)
-(*         rewrite (list_to_set_cons _ qs''). simpl. *)
-(*         apply le_INR. apply subseteq_size. set_solver. *)
-(*       } *)
-(*       iDestruct (ecm_split with "ε") as "[kε ε]". 1,2: real_solver. *)
-(*       iDestruct (ec_split with "δ") as "[kδ δ]". 1,2: real_solver. *)
-(*       rewrite /exact_cache_offline_body... tp_bind (f' _) ; wp_bind (f _). *)
-(*       iCombine "fresh" as "h". *)
-(*       iSpecialize ("h" $! q' cache ε δ _ h M_dipr_q' with "ε δ F rhs"). *)
-(*       iApply (wp_strong_mono'' with "h"). *)
-(*       iIntros "/= %vq' (F & rhs) /=". *)
-(*       rewrite /list_cons... rewrite -/list_cons. *)
-(*       iSpecialize ("IH" $! qs (qs_pre ++ [q']) qs'' QS'' (InjRV (vq', acc)) _). *)
-(*       iSpecialize ("IH" $! _ _ _ _ _ _) => //. *)
-(*       iSpecialize ("IH" with "[kε kδ rhs $F]") => //. *)
-(*       2: iApply "IH" => //. iFrame. *)
-(*       iSplitL "kε" ; [|iSplitL "kδ"]. 3: iSplit ; done. *)
-(*       + iApply ecm_eq. 2: iFrame. real_solver_partial. subst k. simpl. subst k'. *)
-(*         replace (INR $ size (<[q' := vq']> cache)) with (size cache + 1) => //. *)
-(*         rewrite map_size_insert_None => //. qify_r ; zify_q. lia. *)
-(*       + iApply ec_eq. 2: iFrame. real_solver_partial. subst k. simpl. subst k'. *)
-(*         replace (INR $ size (<[q' := vq']> cache)) with (size cache + 1) => //. *)
-(*         rewrite map_size_insert_None => //. qify_r ; zify_q. lia. *)
-(*         Unshelve. *)
-(*         1: subst ; by rewrite cons_middle assoc. *)
-(*         all: subst ; assumption || set_solver. *)
-(*   Qed. *)
+  Definition oxc_spec0_fresh (M : val) c `(dDB : Distance DB) `{Inject A val} `(eqA : Equiv A)
+    (f f' : val) (F : gmap nat A → gmap nat A → iProp Σ) : iProp Σ :=
+    (∀ (q : nat) m m' ε δ K,
+        ⌜m ≡ m'⌝ -∗
+        ⌜q ∉ dom m⌝ -∗
+        wp_diffpriv (M #q) ε δ dDB eqA -∗
+        ↯m (c * ε) -∗
+        ↯ (c * δ) -∗
+        F m m' -∗
+        ⤇ fill K (Val f' #q) -∗
+        WP (Val f) #q {{ v, ∃ (a a' : A), ⌜v = inject a⌝ ∗ ⌜a ≡ a'⌝ ∗ F (<[q := a]> m) (<[q := a']> m') ∗ ⤇ fill K (inject a') }}).
 
 
-(*   (* We can also prove the map variant of the offline exact_cache_dipr from the online spec *) *)
-(*   (* This proof uses induction on the list of queries, which is a bit simpler than direct Löb induction. *) *)
-(*   Lemma exact_cache_dipr_offline_map (M : val) DB (dDB : Distance DB) (qs : list nat) (QS : val) (is_qs : is_list qs QS) *)
-(*     ε δ (εpos : 0 <= ε) (δpos : 0 <= δ) *)
-(*     (M_dipr : Forall (λ q : nat, ⊢ wp_diffpriv (M #q) ε δ dDB) qs) *)
-(*     : *)
-(*     let k := size ((list_to_set qs) : gset _) in *)
-(*     ⊢ wp_diffpriv (exact_cache_offline_map M QS) (k*ε) (k*δ) dDB. *)
-(*   Proof with (tp_pures ; wp_pures). *)
-(*     iIntros (k K c db db' adj) "[rhs [ε δ]]". *)
-(*     rewrite /exact_cache_offline_map... *)
-(*     tp_bind (online_xcache _ _) ; wp_bind (online_xcache _ _). *)
-(*     iPoseProof (oxc_spec0 M _ _ _ _ with "rhs") as "oXC" => //. *)
-(*     iApply (wp_strong_mono'' with "oXC"). *)
-(*     iIntros "%f (%f' & rhs & %F & F & #cached & #fresh) /="... *)
-(*     (* strengthen the postcondition with the resources for the cache & size information for the credits *) *)
-(*     cut *)
-(*       ( ∀ K, {{{ ↯m (c * (k * ε)) ∗ ↯ (c * (k * δ)) ∗ *)
-(*                  □ oxc_spec0_cached f f' F ∗ *)
-(*                  □ oxc_spec0_fresh M c dDB f f' F ∗ *)
-(*                  ⤇ fill K (list_map f' QS) ∗ F ∅ }}} *)
-(*                list_map f QS *)
-(*                {{{ vl, RET vl ; *)
-(*                    ∃ (vr : val) (lvl lvr : list val) cache_qs, *)
-(*                      ⌜is_list lvl vl⌝ ∗ ⌜is_list lvr vr⌝ ∗ ⌜dom cache_qs = list_to_set qs⌝ ∗ *)
-(*                      ⤇ fill K vr ∗ F cache_qs ∗ ⌜vl = vr⌝ }}} ). *)
-(*     { intros h. intros. iApply (h ∅ with "[-]") => //. 1: iFrame. 1: by iSplit. *)
-(*       iNext ; iIntros (?) "(% & % & % & % & % & % & % & rhs & F & %)" ; subst ; done. } *)
-(*     revert QS is_qs. iInduction qs as [|q' qs'] "IH" ; iIntros (QS is_qs). *)
-(*     - iIntros (K' φ). iIntros "(ε & δ & #? & #? & rhs & F) hφ". *)
-(*       simpl in is_qs. subst. rewrite /list_map... simplify_eq. iApply "hφ". iFrame. iExists [],[]. *)
-(*       iPureIntro. intuition auto ; done. *)
-(*     - iIntros (K' φ). iIntros "(ε & δ & #cached & #fresh & rhs & F) hφ". set (qs := q' :: qs'). *)
-(*       rewrite {4}/list_map... rewrite -/list_map. rewrite {3}/list_map... rewrite -!/list_map. *)
-(*       destruct is_qs as (QS' & -> & is_qs')... *)
-(*       destruct (Forall_cons_1 _ _ _ M_dipr) as [M_dipr_q' M_dipr_qs']. *)
-(*       assert (0 <= dDB db db') by apply distance_pos. *)
-(*       tp_bind (list_map f' _) ; wp_bind (list_map f _). *)
-(*       iSpecialize ("IH" $! M_dipr_qs' QS' is_qs' _). *)
-(*       destruct_decide (make_decision (q' ∈ qs')) as cache_q'. *)
-(*       + subst k. assert (list_to_set qs = list_to_set qs') as ->. { subst qs. simpl. set_solver. } *)
-(*         iSpecialize ("IH" with "[-hφ]"). { iFrame. iSplit ; done. } *)
-(*         iApply ("IH"). iIntros "!> %vl (%vr & %lvl & %lvr & %cache_qs' & %is_vl & %is_vr & %dom_cache_qs' & rhs & F & %eqv)". *)
-(*         iSimpl in "rhs"... tp_bind (f' _) ; wp_bind (f _). *)
-(*         unshelve iSpecialize ("cached" $! q' cache_qs' _ _ with "F rhs"). { rewrite dom_cache_qs'. set_solver. } *)
-(*         iApply (wp_strong_mono'' with "cached"). iIntros "/= %v' (F & rhs & %cache_q'')". *)
-(*         rewrite /list_cons... iApply "hφ". iFrame. iModIntro. iPureIntro. simpl. *)
-(*         eexists (v' :: lvl), (v' :: lvr). intuition auto. *)
-(*         * simpl. eexists _. intuition auto. *)
-(*         * simpl. eexists _. intuition auto. *)
-(*         * set_solver. *)
-(*         * subst. done. *)
-(*       + set (k' := size (list_to_set qs' : gset _)). *)
-(*         assert ((k = 1 + k')%nat) as ->. *)
-(*         { subst k. simpl list_to_set. rewrite size_union. 1: rewrite size_singleton ; lia. set_solver. } *)
-(*         assert (∀ α, c * ((1 + k')%nat * α) = c * α + c * (k' * α)) as eq_err ; [|rewrite !eq_err]. *)
-(*         1:{ real_solver_partial. rewrite plus_INR INR_1. field. } *)
-(*         iDestruct (ecm_split with "ε") as "[ε k'ε]" ; [real_solver|real_solver|]. *)
-(*         iDestruct (ec_split with "δ") as "[δ k'δ]" ; [real_solver|real_solver|]. *)
-(*         iSpecialize ("IH" with "[-hφ ε δ]"). { iFrame. iSplit ; done. } *)
-(*         iApply "IH". iIntros "!> %vl (%vr & %lvl & %lvr & %cache_qs' & %is_vl & %is_vr & %dom_cache_qs' & rhs & F & %eqv)". *)
-(*         iSimpl in "rhs"... tp_bind (f' _) ; wp_bind (f _). *)
-(*         unshelve iSpecialize ("fresh" $! q' cache_qs' ε δ _ _ M_dipr_q' with "ε δ F rhs"). *)
-(*         { rewrite dom_cache_qs'. set_solver. } *)
-(*         iApply (wp_strong_mono'' with "fresh"). iIntros "/= %v' (F & rhs)". *)
-(*         rewrite /list_cons... iApply "hφ". iFrame. iModIntro. iPureIntro. simpl. *)
-(*         eexists (v' :: lvl), (v' :: lvr). intuition auto. *)
-(*         * simpl. eexists _. intuition auto. *)
-(*         * simpl. eexists _. intuition auto. *)
-(*         * set_solver. *)
-(*         * subst. done. *)
-(*   Qed. *)
+  #[local] Definition exact_cache_body `{Inject DB val} (M : val) (db : DB) (cache_loc : loc) : expr :=
+    ((λ: "acc" "q",
+        match: get #cache_loc "q" with
+          InjL <> =>
+            let: "v" := M "q" (inject db) in
+            set #cache_loc "q" "v";; list_cons "v" "acc"
+        | InjR "v" => list_cons "v" "acc"
+        end)%V).
 
-(* End xcache. *)
+  Lemma map_equiv_lookup_None `{Countable A} `{Equiv B} (m m' : gmap A B) (a : A) :
+    m ≡ m' → m !! a = None → m' !! a = None.
+  Proof.
+    intros Heq.
+    pose proof lookup_proper a m m' Heq as Hl.
+    destruct (m !! a), (m' !! a); try done.
+    by apply Some_equiv_eq in Hl as (? & ? & ?).
+  Qed.
+
+  (* Direct proof via Löb induction for the definition with fold. *)
+  Lemma exact_cache_dipr (M : val) `(dDB : Distance DB) `(Inject A val) (eqA : Equiv A)
+    (qs : list nat) (QS : val) (is_qs : is_list qs QS) ε δ (εpos : 0 <= ε) (δpos : 0 <= δ)
+    (M_dipr : Forall (λ q : nat, ⊢ hoare_diffpriv (M #q) ε δ dDB (≡@{A})) qs)
+    :
+    let k := size ((list_to_set qs) : gset _) in
+    ⊢ hoare_diffpriv (exact_cache M QS) (k*ε) (k*δ) dDB (≡@{list A}).
+  Proof with (tp_pures ; wp_pures).
+    iIntros (k K c db db' adj φ) "!> [rhs ε] hφ". rewrite {2}/exact_cache...
+    wp_apply wp_init_map => // ; iIntros (cache_l) "cache_l"...
+    rewrite /exact_cache... tp_bind (init_map _).
+    iMod (spec_init_map with "rhs") as "(%cache_r & rhs & cache_r)" => /=...
+    rewrite -!/(exact_cache_body _ _ _).
+    revert qs QS is_qs k M_dipr.
+    cut
+      (∀ (qs : list nat)
+         (qs_pre qs' : list nat) (QS' : val)
+         (acc acc' : list A)
+         (cache_map_l cache_map_r : gmap nat A),
+          qs = qs_pre ++ qs' →
+          acc ≡ acc' →
+          cache_map_l ≡ cache_map_r →
+          dom cache_map_l = list_to_set qs_pre →
+          dom cache_map_l ∪ list_to_set qs' = list_to_set qs →
+          is_list qs' QS' →
+          Forall (λ q : nat, ⊢ hoare_diffpriv (M #q) ε δ dDB (≡@{A})) qs →
+          let k := size (list_to_set qs : gset nat) in
+          let k' := size cache_map_l in
+          {{{
+                ↯m (c * ((k - k') * ε)) ∗ ↯ (c * ((k - k') * δ))
+                ∗ ⤇ fill K (list_fold (exact_cache_body M db' cache_r) (inject acc') QS')
+                ∗ map_list cache_l (inject <$> cache_map_l)
+                ∗ map_slist cache_r (inject <$> cache_map_r)
+          }}}
+            list_fold (exact_cache_body M db cache_l) (inject acc) QS'
+            {{{ (l l' : list A), RET (inject l); ⌜l ≡ l'⌝ ∗ ⤇ fill K (inject l') }}}
+      ).
+    {
+      intros h. intros. iApply (h qs [] qs QS [] [] ∅ ∅ with "[-hφ]") => //.
+      { constructor. }
+      { by apply map_empty_equiv_eq. }
+      { set_solver. }
+      iFrame. rewrite map_size_empty. rewrite Rminus_0_r. subst k. simpl. iFrame.
+    }
+    clear φ.
+    iLöb as "IH".
+    iIntros (qs qs_pre qs' QS' acc acc' cache cache' qs_pre_qs' acc_equiv_acc' dom_cache_pre cacheeq dom_cache_qs'_qs is_qs'
+               M_dipr φ) "(ε & δ & rhs & cache_l & cache_r) hφ /=".
+    set (k := size (list_to_set qs : gset nat)).
+    set (k' := size cache).
+    tp_rec; tp_pures. rewrite -!/(exact_cache_body _ _ _).
+    wp_rec; wp_pures. rewrite -!/(exact_cache_body _ _ _).
+    destruct qs' as [|q' qs''] eqn:qs'_qs''.
+    { rewrite is_qs'. tp_pures. wp_pures. iApply "hφ". iFrame. iModIntro. done. }
+    destruct is_qs' as (QS'' & -> & is_qs'').
+    tp_pures. rewrite -!/(exact_cache_body _ _ _).
+    wp_pures. rewrite -!/(exact_cache_body _ _ _).
+    wp_apply (wp_get with "cache_l"). iIntros (?) "[cache_l ->]".
+    tp_bind (get _ _). iMod (spec_get with "cache_r rhs") as "[rhs cache_r]" => /=.
+    rewrite qs_pre_qs' in M_dipr.
+    destruct ((proj1 (List.Forall_app _ _ _)) M_dipr) as [M_dipr_qs_pre M_dipr_qs'].
+    destruct (Forall_cons_1 _ _ _ M_dipr_qs') as [M_dipr_q' M_dipr_qs''].
+    assert (0 <= dDB db db') by apply distance_pos.
+    destruct (cache !! q') eqn:cache_q' => /=.
+    - opose proof (elem_of_dom_2 _ _ _ cache_q') as h...
+      assert (∃ a', cache' !! q' = Some a' ∧ a ≡ a') as (a' & cache'_q' & a_eq).
+      { by eapply map_equiv_lookup_l. }
+      rewrite !lookup_fmap cache_q' cache'_q' /=.
+      rewrite /list_cons.
+      wp_pures. tp_pures. rewrite -!/(exact_cache_body _ _ _).
+      iSpecialize ("IH" $! qs (qs_pre ++ [q']) qs'' QS'' (a :: acc) (a' :: acc') cache cache').
+      iApply ("IH" with "[%] [%] [%] [%] [%] [%] [%] [$ε $δ $rhs $cache_l $cache_r]") => //; subst.
+      { rewrite cons_middle assoc //. }
+      { by constructor. }
+      { rewrite cacheeq. set_solver. }
+      { rewrite cacheeq. set_solver. }
+      done.
+    - opose proof (not_elem_of_dom_2 _ _ cache_q') as h.
+      rewrite !lookup_fmap cache_q'.
+      assert (cache' !! q' = None) as -> => /=.
+      { by eapply map_equiv_lookup_None. }
+      tp_pures. wp_pures.
+      tp_bind (M _ _). wp_bind (M _ _).
+      assert ((c * ((k - k') * ε)) = (c * (k - (k'+1)) * ε + c * ε)) as -> by lra.
+      assert ((c * ((k - k') * δ)) = (c * (k - (k'+1)) * δ + c * δ)) as -> by lra.
+      assert (0 <= k - (k' + 1)).
+      {
+        subst. subst k k'. apply Rle_0_le_minus.
+        rewrite -dom_cache_qs'_qs.
+        replace (size cache) with (size (dom cache)) by apply size_dom.
+        rewrite dom_cache_pre. replace 1 with (INR 1) by auto.
+        replace 1%nat with (size (list_to_set [q'] : gset nat)).
+        2:{ cbn. rewrite union_empty_r_L. apply size_singleton. }
+        rewrite -plus_INR. rewrite -size_union.
+        { rewrite (list_to_set_cons _ qs''). simpl.
+          apply le_INR. apply subseteq_size. set_solver. }
+        rewrite list_to_set_singleton.
+        rewrite -(dom_proper_L cache cache' dom_cache_pre).
+        set_solver.
+      }
+      iDestruct (ecm_split with "ε") as "[kε ε]". 2: real_solver. 1: repeat real_solver_partial => //.
+      iDestruct (ec_split with "δ") as "[kδ δ]". 2: real_solver. 1: repeat real_solver_partial => //.
+      iApply (M_dipr_q' with "[] [rhs ε δ]") => // ; iFrame. iNext. iIntros (a a') "[% rhs]" => /=...
+      tp_bind (set _ _ _). iMod (spec_set with "cache_r rhs") as "[rhs cache_r]".
+      wp_apply (wp_set with "cache_l") ; iIntros "cache_l"...
+      rewrite /list_cons. do 7 wp_pure. simpl. do 9 tp_pure. rewrite -!/(exact_cache_body _ _ _).
+      rewrite -2!fmap_insert.
+      iSpecialize ("IH" $! qs (qs_pre ++ [q']) qs'' QS'' (a :: _) (a' :: _) ).
+      iApply ("IH" with "[%] [%] [%] [%] [%] [%] [%] [kε kδ $rhs $cache_l $cache_r]") => //; subst.
+      { rewrite cons_middle assoc //. }
+      { by constructor. }
+      { by f_equiv. }
+      { set_solver. }
+      { set_solver. }
+      { done. }
+      iSplitL "kε".
+      + iApply ecm_eq. 2: iFrame. real_solver_partial. subst k. simpl. subst k'.
+        replace (INR $ size (<[q' := _]> cache)) with (size cache + 1) => //.
+        rewrite map_size_insert_None => //. qify_r ; zify_q. lia.
+      + iApply ec_eq. 2: iFrame. real_solver_partial. subst k. simpl. subst k'.
+        replace (INR $ size (<[q' := _]> cache)) with (size cache + 1) => //.
+        rewrite map_size_insert_None => //. qify_r ; zify_q. lia.
+  Qed.
+
+  (* pay as you go, cache map exposed, M only needs to be private on the queries it gets executed on *)
+  Lemma oxc_spec0 (M : val) `(dDB : Distance DB) `{Inject A val} (eqA : Equiv A) `{!Reflexive eqA}
+    (db db' : DB) c (adj : dDB db db' <= c) K :
+    ⤇ fill K (online_xcache M (Val (inject db')))
+    ⊢ WP online_xcache M (Val (inject db))
+        {{ f, ∃ f', ⤇ fill K (Val f') ∗
+                    ∃ (F : gmap nat A → gmap nat A → iProp Σ),
+                      F ∅ ∅ ∗
+                      □ oxc_spec0_cached eqA f f' F ∗
+                      □ oxc_spec0_fresh M c dDB eqA f f' F
+        }}.
+  Proof with (tp_pures ; wp_pures).
+    iIntros "rhs". rewrite /online_xcache...
+    tp_bind (init_map _). iMod (spec_init_map with "rhs") as "[%cache_r [rhs cache_r]]".
+    simpl... wp_apply wp_init_map => //. iIntros (cache_l) "?"...
+    iModIntro. iExists _. iFrame "rhs".
+    iExists (λ m m', map_list cache_l (inject <$> m) ∗ map_slist cache_r (inject <$> m'))%I.
+    iFrame. iSplit.
+    - iIntros "!>" (????? cached ) "[cache_l cache_r] rhs"...
+      tp_bind (get _ _). iMod (spec_get with "[$cache_r] [$rhs]") as "[rhs cache_r]".
+      wp_apply (wp_get with "cache_l") ; iIntros (vq) "[cache_l %hvq]".
+      simpl. subst. apply elem_of_dom in cached. rewrite /opt_to_val.
+      rewrite !lookup_fmap.
+      destruct cached as [vq Hvq] => /=. rewrite Hvq.
+      assert (∃ vq', m' !! q = Some vq' ∧ vq ≡ vq') as (vq' & Hvq' & vq_eq).
+      { by eapply map_equiv_lookup_l. }
+      rewrite Hvq'.
+      tp_pures. wp_pures. iFrame. eauto.
+    - iIntros "!>" (??????? cached) "M_dipr ε δ [cache_l cache_r] rhs"...
+      tp_bind (get _ _). iMod (spec_get with "[$cache_r] [$rhs]") as "[rhs cache_r]".
+      wp_apply (wp_get with "cache_l") ; iIntros (vq) "[cache_l %hvq]".
+      simpl. subst. apply not_elem_of_dom_1 in cached. rewrite /opt_to_val.
+      rewrite !lookup_fmap.
+      assert (m' !! q = None) as -> by by eapply map_equiv_lookup_None.
+      rewrite !cached... tp_bind (M _ _). wp_bind (M _ _).
+      rewrite /wp_diffpriv. iSpecialize ("M_dipr" $! _ c db db' adj).
+      iSpecialize ("M_dipr" with "[$rhs $ε $δ]").
+      iApply (wp_strong_mono'' with "M_dipr"). iIntros (vq) "(%a & %a' & -> & % & rhs)" => /=...
+      tp_bind (set _ _ _). iMod (spec_set with "[$cache_r] [$rhs]") as "[rhs cache_r]".
+      wp_apply (wp_set with "cache_l") ; iIntros "cache_l".
+      simpl. tp_pures. wp_pures. iExists a, a'. rewrite -!fmap_insert. iFrame "∗ %". done.
+  Qed.
+
+  (* we can derive spec1 from spec0 *)
+  (* F can store error credits ; could also ask for N*ε error credits upfront and hand out F(∅, N) instead of F(∅, 0). *)
+  Lemma oxc_spec1 (M : val) `(dDB : Distance DB) `{Inject A val} (eqA : Equiv A) `{!Reflexive eqA} (db db' : DB)
+    (adj : dDB db db' <= 1) K ε δ (εpos : 0 <= ε) (δpos : 0 <= δ) :
+    (∀ q : nat, hoare_diffpriv (M #q) ε δ dDB eqA) ∗
+    ⤇ fill K (online_xcache M (Val (inject db')))
+    ⊢ WP online_xcache M (Val (inject db))
+        {{ f, ∃ f', ⤇ fill K (Val f') ∗
+                    ∃ (F : gmap nat A * gmap nat A * nat → iProp Σ),
+                      F (∅, ∅, 0%nat) ∗
+                      □ (∀ m m' k, ↯m ε ∗ ↯ δ ∗ F(m, m', k) -∗ F(m, m', S k)) ∗
+                      □ (∀ (q : nat) m m' K (N : nat),
+                            ⌜m ≡ m'⌝ -∗
+                            ⌜q ∈ dom m⌝ -∗
+                            F (m, m', N) -∗
+                            ⤇ fill K (Val f' #q) -∗
+                            WP (Val f) #q {{ v, ∃ (a a' : A), ⌜v = inject a⌝ ∗ F(m, m', N) ∗ ⤇ fill K (inject a') ∗  ⌜m !! q = Some a⌝ }}) ∗
+                      □ (∀ (q : nat) m m' K (N : nat),
+                            ⌜m ≡ m'⌝ -∗
+                            ⌜q ∉ dom m⌝ -∗
+                            F(m, m', S N) -∗
+                            ⤇ fill K (Val f' #q) -∗
+                            WP (Val f) #q {{ v, ∃ (a a' : A), ⌜v = inject a⌝ ∗ F (<[q := a]> m, <[q := a']> m', N) ∗ ⤇ fill K (inject a') }})
+        }}.
+  Proof with (tp_pures ; wp_pures).
+    iIntros "(#M_dipr & rhs)". iPoseProof (oxc_spec0 with "rhs") as "spec0" => //.
+    iMod ecm_zero as "ε0" ; iMod ec_zero as "δ0".
+    iApply (wp_strong_mono'' with "spec0"). iIntros "%f (%f' & rhs & (%F & F0 & #f_cached & #f_fresh))".
+    iExists f'. iFrame "rhs".
+    iExists (λ mk : gmap nat A * gmap nat A * nat, let '(m, m', k) := mk in F m m' ∗ ↯m (k * ε) ∗ ↯ (k * δ))%I.
+    rewrite !Rmult_0_l. iFrame "F0 ε0 δ0".
+    iSplitR ; [|iSplitL "f_cached"].
+    - iIntros "!>" (???) "(ε&δ&?&kε&kδ)". iFrame. iPoseProof (ecm_combine with "[ε kε]") as "ε" ; iFrame.
+      iPoseProof (ec_combine with "[δ kδ]") as "δ" ; iFrame. iSplitL "ε".
+      + iApply ecm_eq. 2: iFrame. replace (S k) with (k+1)%nat by lia. replace (INR (k+1)) with (k+1)%R.
+        2: real_solver. lra.
+      + iApply ec_eq. 2: iFrame. replace (S k) with (k+1)%nat by lia. replace (INR (k+1)) with (k+1)%R.
+        2: real_solver. lra.
+    - simpl. iIntros "!>" (???????) "[FA [ε δ]] rhs". iSpecialize ("f_cached" with "[//] [//] [$FA] [$rhs]").
+      iApply (wp_strong_mono'' with "f_cached"). iIntros (?) "(%a & %a' & -> & % & FA & rhs & ?)". iFrame => //.
+    - iIntros "!>" (???????) "[FA [ε δ]] rhs".
+      replace ((S N)) with (N + 1)%nat by lia. replace (INR (N+1)) with (N+1) by real_solver.
+      rewrite !Rmult_plus_distr_r. rewrite !Rmult_1_l.
+      iDestruct (ecm_split with "ε") as "[Nε ε]". 1,2: real_solver.
+      iDestruct (ec_split with "δ") as "[Nδ δ]". 1,2: real_solver.
+      iSpecialize ("f_fresh" with "[//] [//] [] [ε] [δ] [$FA] [$rhs]").
+      { iIntros (?????) "[??]". iApply ("M_dipr" with "[//] [$]").
+        iIntros "!>" (??) "[$ $] //". }
+      1,2: rewrite Rmult_1_l => //.
+      iApply (wp_strong_mono'' with "f_fresh").
+      iIntros (?) "(%a & %a' & -> & % & FA & rhs)". iFrame => //.
+  Qed.
+
+  (* We can prove exact_cache_dipr from the online spec. The proof is essentially the same as the direct proof. *)
+  Lemma exact_cache_dipr_offline (M : val) DB (dDB : Distance DB) `{Inject A val} (eqA : Equiv A) `{!Reflexive eqA}
+    (qs : list nat) (QS : val) (is_qs : is_list qs QS)
+    ε δ (εpos : 0 <= ε) (δpos : 0 <= δ)
+    (M_dipr : Forall (λ q : nat, ⊢ wp_diffpriv (M #q) ε δ dDB (≡@{A})) qs)
+    :
+    let k := size ((list_to_set qs) : gset _) in
+    ⊢ wp_diffpriv (exact_cache_offline M QS) (k*ε) (k*δ) dDB (≡@{list A}).
+  Proof with (tp_pures ; wp_pures).
+    iIntros (k K c db db' adj) "[rhs [ε δ]]".
+    rewrite {2}/exact_cache_offline...
+    rewrite /exact_cache_offline...
+    tp_bind (online_xcache _ _). wp_bind (online_xcache _ _).
+    iPoseProof (oxc_spec0 M _ _ _ _) as "oXC" => //.
+    iSpecialize ("oXC" with "rhs").
+    iApply (wp_strong_mono'' with "oXC").
+    iIntros "%f (%f' & rhs & %F & F & #cached & #fresh) /="...
+    set (exact_cache_offline_body (f : val) := (λ: "acc" "q", list_cons (f "q") "acc")%V).
+    rewrite -!/(exact_cache_offline_body _).
+    revert qs QS is_qs k M_dipr.
+    cut
+      (∀ (qs : list nat)
+         (qs_pre qs' : list nat) (QS' : val)
+         (acc acc' : list A) cache_map_l cache_map_r,
+          acc ≡ acc' →
+          cache_map_l ≡ cache_map_r →
+          qs = qs_pre ++ qs' →
+          dom cache_map_l = list_to_set qs_pre →
+          dom cache_map_l ∪ list_to_set qs' = list_to_set qs →
+          is_list qs' QS' →
+          Forall (λ q : nat, ⊢ wp_diffpriv (M #q) ε δ dDB (≡@{A})) qs →
+          let k := size (list_to_set qs : gset nat) in
+          let k' := size cache_map_l in
+          {{{
+                ↯m (c * ((k - k') * ε)) ∗ ↯ (c * ((k - k') * δ)) ∗
+                □ oxc_spec0_cached eqA f f' F ∗
+                □ oxc_spec0_fresh M c dDB eqA f f' F ∗
+                ⤇ fill K (list_fold (exact_cache_offline_body f') (inject acc') QS') ∗
+                F cache_map_l cache_map_r
+          }}}
+            list_fold (exact_cache_offline_body f) (inject acc)%V QS'
+          {{{ (l l' : list A), RET (inject l); ⌜l ≡ l'⌝ ∗ ⤇ fill K (inject l') }}}
+      ).
+    {
+      intros h. intros. iApply (h qs [] qs QS [] [] ∅ ∅ with "[-]") => //.
+      { constructor. }
+      { by apply map_empty_equiv_eq. }
+      { set_solver. }
+      { iFrame. rewrite map_size_empty. rewrite Rminus_0_r. subst k. simpl. iFrame "∗ #". }
+      by iIntros "!>" (??) "($ & $)".
+    }
+    iLöb as "IH".
+    iIntros (qs qs_pre qs' QS' acc acc' cache_l cache_r accs caches qs_pre_qs' dom_cache_pre dom_cache_qs'_qs is_qs'
+               M_dipr φ) "(ε & δ & #cached & #fresh & rhs & F) hφ".
+    set (k := size (list_to_set qs : gset nat)).
+    set (k' := size cache_l).
+    rewrite /exact_cache_offline_body /=.
+    tp_rec. tp_pures.
+    wp_rec. wp_pures.
+    destruct qs' as [|q' qs''] eqn:qs'_qs''.
+    { rewrite is_qs'. tp_pures. wp_pures. iApply "hφ". iModIntro. iFrame "∗ %". }
+    destruct is_qs' as (QS'' & -> & is_qs'').
+    tp_pures. wp_pures.
+    rewrite qs_pre_qs' in M_dipr.
+    destruct ((proj1 (List.Forall_app _ _ _)) M_dipr) as [M_dipr_qs_pre M_dipr_qs'].
+    destruct (Forall_cons_1 _ _ _ M_dipr_qs') as [M_dipr_q' M_dipr_qs''].
+    assert (0 <= dDB db db') by apply distance_pos.
+    destruct (cache_l !! q') eqn:cache_q' => /=.
+    - opose proof (elem_of_dom_2 _ _ _ cache_q') as h...
+      tp_bind (f' _) ; wp_bind (f _).
+      iCombine "cached" as "h".
+      iSpecialize ("h" $! q' cache_l cache_r _ _ h with "F rhs").
+      iApply (wp_strong_mono'' with "h").
+      iIntros "/= %v' (%b & %b' & -> & % & F & rhs & %cache_q'')".
+      assert (a = b) as <-. { rewrite cache_q' in cache_q''. inversion cache_q''. done. }
+      tp_rec. wp_rec. tp_pures. wp_pures.
+      iSpecialize ("IH" $! qs (qs_pre ++ [q']) qs'' QS'' (_ :: _) (_ :: _) cache_l cache_r).
+      iApply ("IH" with "[%] [%] [%] [%] [%] [%] [%] [ε δ rhs F]") => //.
+      { by constructor. }
+      { subst. rewrite cons_middle assoc //. }
+      { set_solver. }
+      { set_solver. }
+      { subst. done. }
+      iFrame "∗ #".
+    - opose proof (not_elem_of_dom_2 _ _ cache_q') as h...
+      assert ((c * ((k - k') * ε)) = (c * (k - (k'+1)) * ε + c * ε)) as -> by lra.
+      assert ((c * ((k - k') * δ)) = (c * (k - (k'+1)) * δ + c * δ)) as -> by lra.
+      assert (0 <= k - (k' + 1)).
+      {
+        subst. subst k k'. apply Rle_0_le_minus.
+        rewrite -dom_cache_qs'_qs.
+        replace (size cache_l) with (size (dom cache_l)) by apply size_dom.
+        rewrite dom_cache_pre. replace 1 with (INR 1) by auto.
+        replace 1%nat with (size (list_to_set [q'] : gset nat)).
+        2:{ cbn. rewrite union_empty_r_L. apply size_singleton. }
+        rewrite -plus_INR. rewrite -size_union. 2: set_solver.
+        rewrite (list_to_set_cons _ qs''). simpl.
+        apply le_INR. apply subseteq_size. set_solver.
+      }
+      iDestruct (ecm_split with "ε") as "[kε ε]". 1,2: real_solver.
+      iDestruct (ec_split with "δ") as "[kδ δ]". 1,2: real_solver.
+      rewrite /exact_cache_offline_body... tp_bind (f' _) ; wp_bind (f _).
+      iCombine "fresh" as "h".
+      iSpecialize ("h" $! q' cache_l cache_r ε δ _ caches h M_dipr_q' with "ε δ F rhs").
+      iApply (wp_strong_mono'' with "h").
+      iIntros "/= %vq' (%a & %a' & -> & % & F & rhs) /=".
+      tp_rec. wp_rec. tp_pures. wp_pures.
+      iSpecialize ("IH" $! qs (qs_pre ++ [q']) qs'' QS'' (_ :: _) (_ :: _)).
+      iApply ("IH" with "[%] [%] [%] [%] [%] [%] [%] [kε kδ $rhs $F]") => //.
+      { by constructor. }
+      { by f_equiv. }
+      { subst. rewrite cons_middle assoc //. }
+      { set_solver. }
+      { set_solver. }
+      { subst. done. }
+      iSplitL "kε" ; [|iSplitL "kδ"]. 3: iSplit ; done.
+      + iApply ecm_eq. 2: iFrame. real_solver_partial. subst k. simpl. subst k'.
+        replace (INR $ size (<[q' := _]> cache_l)) with (size cache_l + 1) => //.
+        rewrite map_size_insert_None => //. qify_r ; zify_q. lia.
+      + iApply ec_eq. 2: iFrame. real_solver_partial. subst k. simpl. subst k'.
+        replace (INR $ size (<[q' := _]> cache_l)) with (size cache_l + 1) => //.
+        rewrite map_size_insert_None => //. qify_r ; zify_q. lia.
+     Unshelve. done.
+  Qed.
+
+  (* We can also prove the map variant of the offline exact_cache_dipr from the online spec *)
+  (* This proof uses induction on the list of queries, which is a bit simpler than direct Löb induction. *)
+  Lemma exact_cache_dipr_offline_map (M : val) DB (dDB : Distance DB)  `{Inject A val} (eqA : Equiv A) `{!Reflexive eqA}
+    (qs : list nat) (QS : val) (is_qs : is_list qs QS)
+    ε δ (εpos : 0 <= ε) (δpos : 0 <= δ)
+    (M_dipr : Forall (λ q : nat, ⊢ wp_diffpriv (M #q) ε δ dDB (≡@{A})) qs)
+    :
+    let k := size ((list_to_set qs) : gset _) in
+    ⊢ wp_diffpriv (exact_cache_offline_map M QS) (k*ε) (k*δ) dDB (≡@{list A}).
+  Proof with (tp_pures ; wp_pures).
+    iIntros (k K c db db' adj) "[rhs [ε δ]]".
+    rewrite /exact_cache_offline_map...
+    tp_bind (online_xcache _ _) ; wp_bind (online_xcache _ _).
+    iPoseProof (oxc_spec0 M _ _ _ _ with "rhs") as "oXC" => //.
+    iApply (wp_strong_mono'' with "oXC").
+    iIntros "%f (%f' & rhs & %F & F & #cached & #fresh) /="...
+    (* strengthen the postcondition with the resources for the cache & size information for the credits *)
+    cut
+      ( ∀ K, {{{ ↯m (c * (k * ε)) ∗ ↯ (c * (k * δ)) ∗
+                 □ oxc_spec0_cached eqA f f' F ∗
+                 □ oxc_spec0_fresh M c dDB eqA f f' F ∗
+                 ⤇ fill K (list_map f' QS) ∗ F ∅ ∅ }}}
+               list_map f QS
+               {{{ (l l' : list A), RET (inject l);
+                   ∃ cache_qs cache'_qs,
+                     ⌜l ≡ l'⌝ ∗ ⌜cache_qs ≡ cache'_qs⌝ ∗ ⌜dom cache_qs = list_to_set qs⌝ ∗
+                     ⤇ fill K (inject l') ∗ F cache_qs cache'_qs }}} ).
+    { intros h. intros. iApply (h with "[$]") => //.
+      iNext ; iIntros (??) "(% & % & $ & % & % & $ & F) //".
+    }
+    revert QS is_qs. iInduction qs as [|q' qs'] "IH" ; iIntros (QS is_qs).
+    - iIntros (K' φ). iIntros "(ε & δ & #? & #? & rhs & F) hφ".
+      simpl in is_qs. subst. wp_rec; tp_rec... iApply ("hφ" $! [] []). iFrame. iModIntro. iPureIntro.
+      do 2 (split; [constructor|]). done.
+    - iIntros (K' φ). iIntros "(ε & δ & #cached & #fresh & rhs & F) hφ". set (qs := q' :: qs').
+      tp_rec; wp_rec...
+      destruct is_qs as (QS' & -> & is_qs')...
+      destruct (Forall_cons_1 _ _ _ M_dipr) as [M_dipr_q' M_dipr_qs'].
+      assert (0 <= dDB db db') by apply distance_pos.
+      tp_bind (list_map f' _) ; wp_bind (list_map f _).
+      iSpecialize ("IH" $! M_dipr_qs' QS' is_qs' _).
+      destruct (decide (q' ∈ qs')) as [cache_q'|cache_q'].
+      + subst k. assert (list_to_set qs = list_to_set qs') as ->. { subst qs. simpl. set_solver. }
+        iSpecialize ("IH" with "[-hφ]"). { iFrame. iSplit ; done. }
+        iApply ("IH").
+        iIntros "!>" (l l') "(%cache_qs & %cache_qs' & % & %cache_eq & %dom_cache_qs & rhs & F)".
+        iSimpl in "rhs"... tp_bind (f' _) ; wp_bind (f _).
+        iSpecialize ("cached" $! q' cache_qs cache_qs' with "[//] [%] F rhs").
+        { rewrite dom_cache_qs. set_solver. }
+        iApply (wp_strong_mono'' with "cached"). iIntros "/= %v' (%a & %a' & -> & % & F & rhs & %cache_q'')".
+        rewrite /list_cons... iApply ("hφ" $! (_ :: _) (_ :: _)). iFrame. iModIntro. iPureIntro.
+        split; [by f_equiv|].
+        split; [done|].
+        set_solver.
+      + set (k' := size (list_to_set qs' : gset _)).
+        assert ((k = 1 + k')%nat) as ->.
+        { subst k. simpl list_to_set. rewrite size_union. 1: rewrite size_singleton ; lia. set_solver. }
+        assert (∀ α, c * ((1 + k')%nat * α) = c * α + c * (k' * α)) as eq_err ; [|rewrite !eq_err].
+        1:{ real_solver_partial. rewrite plus_INR INR_1. field. }
+        iDestruct (ecm_split with "ε") as "[ε k'ε]" ; [real_solver|real_solver|].
+        iDestruct (ec_split with "δ") as "[δ k'δ]" ; [real_solver|real_solver|].
+        iSpecialize ("IH" with "[-hφ ε δ]"). { iFrame. iSplit ; done. }
+        iApply "IH".
+        iIntros "!>" (l l') "(%cache_qs & %cache_qs' & % & %cache_eq & %dom_cache_qs & rhs & F)".
+        iSimpl in "rhs"... tp_bind (f' _) ; wp_bind (f _).
+        iSpecialize ("fresh" $! q' cache_qs cache_qs' with "[//] [%] [//] ε δ F rhs").
+        { rewrite dom_cache_qs. set_solver. }
+        iApply (wp_strong_mono'' with "fresh"). iIntros "/= %v' (%a & %a' & -> & % & F & rhs)".
+        wp_rec; tp_rec... iApply ("hφ" $! (_ :: _) (_ :: _)). iFrame. iModIntro. iPureIntro.
+        split; [by f_equiv|].
+        split; [by f_equiv|].
+        set_solver.
+  Qed.
+
+End xcache.
